<?xml version="1.0"?>


<!DOCTYPE rdf:RDF [
    <!ENTITY owl "http://www.w3.org/2002/07/owl#" >
    <!ENTITY xsd "http://www.w3.org/2001/XMLSchema#" >
    <!ENTITY rdfs "http://www.w3.org/2000/01/rdf-schema#" >
    <!ENTITY rdf "http://www.w3.org/1999/02/22-rdf-syntax-ns#" >
    <!ENTITY process "http://www.daml.org/services/owl-s/1.2/Process.owl#" >
    <!ENTITY service "http://www.daml.org/services/owl-s/1.2/Service.owl#" >
    <!ENTITY grounding "http://www.daml.org/services/owl-s/1.2/Grounding.owl#" >
    <!ENTITY sparql-grounding "http://localhost/ontology/sparqlGrounding.owl#" >
    <!ENTITY shadow-rdf "http://www.daml.org/services/owl-s/1.2/generic/ObjectList.owl#" >
]>


<rdf:RDF xmlns="http://localhost/ontology/sparqlGrounding.owl#"
     xmlns:process="http://www.daml.org/services/owl-s/1.2/Process.owl#"
     xmlns:rdfs="http://www.w3.org/2000/01/rdf-schema#"
     xmlns:grounding="http://www.daml.org/services/owl-s/1.2/Grounding.owl#"
     xmlns:service="http://www.daml.org/services/owl-s/1.2/Service.owl#"
     xmlns:owl="http://www.w3.org/2002/07/owl#"
     xmlns:xsd="http://www.w3.org/2001/XMLSchema#"
     xmlns:rdf="http://www.w3.org/1999/02/22-rdf-syntax-ns#"
     xmlns:shadow-rdf="http://www.daml.org/services/owl-s/1.2/generic/ObjectList.owl#">
    <owl:Ontology rdf:about="http://localhost/ontology/sparqlGrounding.owl">
        <rdfs:comment>
        Upper-level OWL ontology for Groundings that employ SPARQL services. Part of the OWL-S ontology; see http://www.daml.org/services/. This version is intended for use with SPARQL 1.1.
        </rdfs:comment>
        <owl:versionInfo>
        $Id: sparqlGrounding.owl,v 1.38 2014/04/17 17:11:56 leandroandrade Exp $
        </owl:versionInfo>
        <owl:imports rdf:resource="http://www.daml.org/services/owl-s/1.2/Process.owl"/>
    </owl:Ontology>
    
    
    <owl:Class rdf:about="&sparql-grounding;SparqlGrounding">
        <rdfs:subClassOf rdf:resource="&grounding;Grounding"/>
        <rdfs:subClassOf>
            <owl:Restriction>
                <owl:onProperty rdf:resource="&grounding;hasAtomicProcessGrounding"/>
                <owl:allValuesFrom rdf:resource="&sparql-grounding;SparqlAtomicProcessGrounding"/>
            </owl:Restriction>
        </rdfs:subClassOf>
        <rdfs:comment>
            The class that grounds every process to a SPARQL query.
        </rdfs:comment>
    </owl:Class>
    
    <owl:Class rdf:about="&sparql-grounding;SparqlAtomicProcessGrounding">
        <rdfs:subClassOf rdf:resource="&grounding;AtomicProcessGrounding"/>
        <rdfs:subClassOf>
            <owl:Restriction>
                <owl:onProperty rdf:resource="&sparql-grounding;sparqlEndPoint"/>
                <owl:cardinality rdf:datatype="&xsd;#nonNegativeInteger">1</owl:cardinality>
            </owl:Restriction>
        </rdfs:subClassOf>
        <rdfs:comment>
            The class that relates elements of an OWL-S atomic process to a SPARQL query.
        </rdfs:comment>
    </owl:Class>
    
    <owl:DatatypeProperty rdf:about="&sparql-grounding;sparqlDocument">
        <rdfs:comment>
            The URI that indicates the SPARQL document to which this grounding refers to.
        </rdfs:comment>
        <rdfs:domain rdf:resource="&sparql-grounding;SparqlAtomicProcessGrounding"/>
        <rdfs:range rdf:resource="&xsd;anyURI"/>
    </owl:DatatypeProperty>

    <owl:DatatypeProperty rdf:about="&sparql-grounding;sparqlEndPoint">
        <rdfs:comment>
            A URI for a SPARQL endpoint that provides the operation to which this atomic process is grounded.
        </rdfs:comment>
        <rdfs:domain rdf:resource="&sparql-grounding;SparqlAtomicProcessGrounding"/>
        <rdfs:range rdf:resource="&xsd;anyURI"/>
    </owl:DatatypeProperty>

    <owl:DatatypeProperty rdf:about="&sparql-grounding;sparqlVersion">
        <rdf:type rdf:resource="&owl;FunctionalProperty"/>
        <rdfs:comment>
            The URI that indicates the SPARQL version being used.
        </rdfs:comment>
        <rdfs:domain rdf:resource="&sparql-grounding;SparqlAtomicProcessGrounding"/>
        <rdfs:range rdf:resource="&xsd;anyURI"/>
    </owl:DatatypeProperty>
    
    <owl:ObjectProperty rdf:about="&sparql-grounding;SparqlInputParam">
        <rdfs:comment>
            There should be one instance of this property for each SPARQL input data.
        </rdfs:comment>
        <rdfs:domain rdf:resource="&sparql-grounding;SparqlAtomicProcessGrounding"/>
        <rdfs:range rdf:resource="&sparql-grounding;SparqlInputParamMap"/>
    </owl:ObjectProperty>

    <owl:ObjectProperty rdf:about="&sparql-grounding;SparqlOutputParam">
        <rdfs:comment>
            There should be one instance of this property for each SPARQL select parameter.
        </rdfs:comment>
        <rdfs:domain rdf:resource="&sparql-grounding;SparqlAtomicProcessGrounding"/>
        <rdfs:range rdf:resource="&sparql-grounding;SparqlOutputParamMap"/>
    </owl:ObjectProperty>
    
    <owl:Class rdf:about="&sparql-grounding;SparqlInputParamMap">
        <rdfs:subClassOf rdf:resource="&grounding;InputMessageMap"/>
        <rdfs:subClassOf rdf:resource="&sparql-grounding;SparqlDataParamMap"/>
        <rdfs:comment>
            The mapping entity that shows how to derive a WADL response message parameter from an OWL-S parameter value.
        </rdfs:comment>
    </owl:Class>

    <owl:Class rdf:about="&sparql-grounding;SparqlOutputParamMap">
        <rdfs:subClassOf rdf:resource="&grounding;OutputMessageMap"/>
        <rdfs:subClassOf rdf:resource="&sparql-grounding;SparqlDataParamMap"/>
        <rdfs:comment>
        The mapping entity that shows how to relate a SPARQL select variable parameter from an OWL-S parameter value.
        </rdfs:comment>
    </owl:Class>
    

    <owl:Class rdf:about="&sparql-grounding;SparqlDataParamMap">
        <rdfs:subClassOf rdf:resource="&grounding;MessageMap"/>
        <rdfs:subClassOf>
            <owl:Restriction>
                <owl:onProperty rdf:resource="&sparql-grounding;SparqlDataParam"/>
                <owl:cardinality rdf:datatype="&xsd;nonNegativeInteger">1</owl:cardinality>
            </owl:Restriction>
        </rdfs:subClassOf>
        <rdfs:subClassOf>
            <owl:Restriction>
                <owl:onProperty rdf:resource="&grounding;owlsParameter"/>
                <owl:cardinality rdf:datatype="&xsd;nonNegativeInteger">1</owl:cardinality>
            </owl:Restriction>
        </rdfs:subClassOf>
    </owl:Class>


    <owl:DatatypeProperty rdf:about="&sparql-grounding;SparqlDataParam">
        <rdfs:comment>
            Message mapping for variables of SPARQL query.
        </rdfs:comment>
        <rdfs:domain rdf:resource="&sparql-grounding;SparqlDataParamMap"/>
        <rdfs:range rdf:resource="&xsd;anyURI"/>
    </owl:DatatypeProperty>
    
    
    <owl:ObjectProperty rdf:about="&sparql-grounding;SparqlPrefixies">
        <rdfs:comment>
            There should be one instance of this property for each SPARQL input data.
        </rdfs:comment>
        <rdfs:domain rdf:resource="&sparql-grounding;SparqlAtomicProcessGrounding"/>
        <rdfs:range rdf:resource="&sparql-grounding;SparqlPrefixMap"/>
    </owl:ObjectProperty>

    <owl:Class rdf:ID="SparqlPrefixMap">
      <rdfs:comment>
            There should be one instance of this property for each SPARQL input data.
        </rdfs:comment>
      <rdfs:subClassOf>
        <owl:Restriction>
          <owl:onProperty rdf:resource="#PrefixName"/>
          <owl:cardinality rdf:datatype="&xsd;nonNegativeInteger">1</owl:cardinality>
        </owl:Restriction>
      </rdfs:subClassOf>
      <rdfs:subClassOf>
        <owl:Restriction>
          <owl:onProperty rdf:resource="#PrefixUri"/>
          <owl:cardinality rdf:datatype="&xsd;nonNegativeInteger">1</owl:cardinality>
        </owl:Restriction>
      </rdfs:subClassOf>
    </owl:Class>

    <owl:DatatypeProperty rdf:ID="PrefixName">
      <rdfs:domain rdf:resource="#WadlResourceMethodRef"/>
      <rdfs:range rdf:resource="&xsd;anyURI"/>
    </owl:DatatypeProperty>

    <owl:DatatypeProperty rdf:ID="PrefixUri">
      <rdfs:domain rdf:resource="#WadlResourceMethodRef"/>
      <rdfs:range rdf:resource="&xsd;string"/>
    </owl:DatatypeProperty>
    
    
    <owl:ObjectProperty rdf:about="&sparql-grounding;SparqlTriples">
        <rdfs:comment>
            There should be one instance of this property for each SPARQL input data.
        </rdfs:comment>
        <rdfs:domain rdf:resource="&sparql-grounding;SparqlAtomicProcessGrounding"/>
        <rdfs:range rdf:resource="&sparql-grounding;SparqlTripleMap"/>
    </owl:ObjectProperty>
    
    <owl:Class rdf:ID="SparqlTripleMap">
      <rdfs:comment>
            There should be one instance of this property for each SPARQL input data.
        </rdfs:comment>
      <rdfs:subClassOf>
        <owl:Restriction>
          <owl:onProperty rdf:resource="#TripleSubject"/>
          <owl:cardinality rdf:datatype="&xsd;nonNegativeInteger">1</owl:cardinality>
        </owl:Restriction>
      </rdfs:subClassOf>
      <rdfs:subClassOf>
        <owl:Restriction>
          <owl:onProperty rdf:resource="#TriplePredicate"/>
          <owl:cardinality rdf:datatype="&xsd;nonNegativeInteger">1</owl:cardinality>
        </owl:Restriction>
      </rdfs:subClassOf>
      <rdfs:subClassOf>
        <owl:Restriction>
          <owl:onProperty rdf:resource="#TripleObject"/>
          <owl:cardinality rdf:datatype="&xsd;nonNegativeInteger">1</owl:cardinality>
        </owl:Restriction>
      </rdfs:subClassOf>
    </owl:Class>
    
    <owl:DatatypeProperty rdf:ID="TripleSubject">
      <rdfs:domain rdf:resource="#WadlResourceMethodRef"/>
      <rdfs:range rdf:resource="&xsd;string"/>
    </owl:DatatypeProperty>

    <owl:DatatypeProperty rdf:ID="TriplePredicate">
      <rdfs:domain rdf:resource="#WadlResourceMethodRef"/>
      <rdfs:range rdf:resource="&xsd;string"/>
    </owl:DatatypeProperty>
    
    <owl:DatatypeProperty rdf:ID="TripleObject">
      <rdfs:domain rdf:resource="#WadlResourceMethodRef"/>
      <rdfs:range rdf:resource="&xsd;string"/>
    </owl:DatatypeProperty>

    

</rdf:RDF>


